src/x86/step.v
@@ -1,9 +1,6 @@
 (*===========================================================================
-    Single-step transition function
-
-    As well as ordinary x86 instruction semantics, this incorporates I/O 
-    actions, which are "faked" by assuming that the semantics of entering 
-    two well-known memory locations is to perform input or output.
+    Single-step transition function and extension to multiple steps,
+    with various lemmas
   ===========================================================================*)
 Require Import ssreflect ssrnat ssrbool eqtype tuple seq. 
 Require Import instr monad reader procstate procstatemonad exn eval instrcodec 
@@ -12,6 +9,16 @@ Require Import instr monad reader procstate procstatemonad exn eval instrcodec
 Set Implicit Arguments.
 Unset Strict Implicit.
 Import Prenex Implicits.
+
+Definition Obs := seq (Chan * Data).
+Definition preObs (o1 o2: Obs) := exists o', o2 = o1 ++ o'.
+
+Require Import RelationClasses Program.Basics.
+Instance preObs_Pre: PreOrder preObs.
+Proof. repeat constructor; hnf.
+move => o. exists nil. by rewrite cats0.
+move => x y z [o1 H1] [o2 H2]. subst. exists (o1++o2). by rewrite catA. 
+Qed. 
 
 (* Decode instruction at EIP, move EIP to next instruction, execute instruction *)
 (*=step *)
@@ -22,6 +29,135 @@ Definition step : ST unit :=
   evalInstr instr.
 (*=End *)
 
+(* Takes one step from s to s' with output o *)
+Definition oneStep s o s' := step s = (o, Success _ (s', tt)). 
 
+(* Takes k steps from s to s' with output o *)
+Definition manyStep k s o s' := doMany k step s = (o, Success _ (s', tt)).
 
+(* Takes at least k steps from s *)
+Definition runsFor k s := exists s' o, manyStep k s o s'.
+Definition runsForWith k o s := exists s', manyStep k o s s'. 
+
+(* Runs forever from s without failing *)
+Definition runsForever s := forall k, runsFor k s.
+
+(* Takes some number of steps from s to s' *)
+Definition runsTo s s' := exists k o, manyStep k s o s'.
+Definition runsToWith s o s' := exists k, manyStep k s o s'. 
+
+(* Takes at least one step from s to s' *)
+Definition properRunsTo s s' := exists k o, manyStep k.+1 s o s'.
+Definition properRunsToWith s o s' := exists k, manyStep k.+1 s o s'. 
+
+Lemma seqManyStep k1 : forall k2 s s' s'' o1 o2,
+  manyStep k1 s o1 s' -> 
+  manyStep k2 s' o2 s'' ->
+  manyStep (k1+k2) s (o1++o2) s''.
+Proof. induction k1 => k2 s s' s'' o1 o2 R1 R2.
++ rewrite add0n. injection R1 => [E1 E2]. by subst. 
++ rewrite /manyStep/= in R1, R2. 
+  elim E1: (step s) => [o'' r]. rewrite E1 in R1. 
+  elim E2: r => [e| [s''' []]]. by rewrite E2 in R1. 
+  rewrite E2 in R1. 
+  elim E3: (doMany k1 step s''') => [o''' r']. rewrite E3 in R1. 
+  injection R1 => [R1a R2b]. subst.   
+  specialize (IHk1 _ _ _ _ _ _ E3 R2). rewrite /manyStep/=. by rewrite E1 IHk1 catA.  
+Qed. 
+
+Lemma runsFor0 s : runsFor 0 s.
+Proof. by exists s, nil. Qed. 
+
+Lemma runsForWith0 s : runsForWith 0 s nil.
+Proof. by exists s. Qed. 
+
+Lemma runsForSinv s k : runsFor k.+1 s ->
+  exists s' o, (oneStep s o s' /\ runsFor k s').
+Proof. rewrite /runsFor. move => [s' [o RED]]. 
+rewrite /manyStep/= in RED. 
+case E1: (step s) => [o'' r]. rewrite E1 in RED. 
+elim E2: r => [e| [s''' []]]. by rewrite E2 in RED. 
+rewrite E2 in RED. 
+exists s''', o''. split. by rewrite /oneStep E1 E2. 
+elim E3: (doMany k step s''') => [o''' r']. rewrite E3 in RED. 
+injection RED => [EQ1 EQ2]. subst.
+rewrite /manyStep E3. by eexists _, _. Qed. 
+
+Lemma runsForWithSinv s k o : runsForWith k.+1 s o ->
+  exists s' o1 o2, (oneStep s o1 s' /\ runsForWith k s' o2 /\ o = o1++o2).
+Proof. rewrite /runsForWith. move => [s' RED]. 
+rewrite /manyStep/= in RED. 
+case E1: (step s) => [o1 r]. rewrite E1 in RED. 
+elim E2: r => [e| [s''' []]]. by rewrite E2 in RED. 
+rewrite E2 in RED. 
+elim E3: (doMany k step s''') => [o''' r']. rewrite E3 in RED.
+exists s''', o1, o'''. split. by rewrite /oneStep E1 E2. 
+injection RED => [EQ1 EQ2]. subst.
+rewrite /manyStep E3. split => //. by eexists. 
+Qed. 
+
+Lemma runsForS k s o s' : oneStep s o s' -> runsFor k s' -> runsFor k.+1 s.
+Proof. move => RED1 RED2. rewrite /oneStep in RED1. 
+destruct RED2 as [s'' [o'' RED2]]. rewrite /runsFor.
+rewrite /manyStep/=. rewrite RED1 RED2. by eexists _, _. 
+Qed. 
+
+Lemma runsForWithS k s o s' o' : 
+  oneStep s o s' -> runsForWith k s' o' -> runsForWith k.+1 s (o++o').
+Proof. move => RED1 [s'' RED2]. rewrite /oneStep in RED1. 
+rewrite /runsForWith.
+rewrite /manyStep/=. rewrite RED1 RED2. by eexists _. 
+Qed. 
+
+Lemma runsForLe k : forall k', k' <= k -> forall s, runsFor k s -> runsFor k' s.
+Proof. induction k => k' LT s RED => //.
++ destruct k' => //. 
++ destruct k' => //. apply runsFor0. 
++ specialize (IHk _ LT). 
+apply runsForSinv in RED. destruct RED as [s' [o [R1 RED]]]. 
+apply: runsForS. apply R1. by apply IHk. 
+Qed. 
+
+Lemma cat_preObs o : forall o1 o2, preObs o1 o2 -> preObs (o++o1) (o++o2). 
+Proof. induction o => // o1 o2 [o' PO]. subst. exists o'. by rewrite catA. Qed.
+
+Lemma runsForWithLe k : forall o k', k' <= k -> forall s, runsForWith k s o -> 
+  exists o', preObs o' o /\ runsForWith k' s o'.
+Proof. induction k => o k' LT s RED => //.
++ destruct k' => //. exists o. split => //. reflexivity. 
++ destruct k' => //. exists nil. split => //. by exists o. apply runsForWith0. 
++ apply runsForWithSinv in RED. destruct RED as [s' [o' [o'' [R1 [RED E]]]]].
+subst. 
+destruct (IHk o'' _ LT _ RED) as [o0 [OBS RUNS]]. 
+exists (o'++o0). split. by apply cat_preObs. 
+apply: runsForWithS. apply R1. done. 
+Qed. 
+
+Lemma runsTo_runsForever s s' :runsTo s s' -> runsForever s' -> runsForever s.
+Proof. 
+move => [k [o RED]] RF k0. 
+case LE: (k <= k0). 
+specialize (RF (k0-k)). 
+destruct RF as [s'' [o' RF]]. 
+have RED1 := seqManyStep RED RF. rewrite subnKC in RED1 => //. eexists _, _. apply RED1.
+have LT: k0 < k. by rewrite ltnNge LE. 
+apply: runsForLe. apply ltnW in LT. apply LT. by exists s', o.
+Qed. 
+
+Lemma runsTo_runsFor k : forall s s', runsTo s s' -> runsFor k s' -> runsFor k s. 
+Proof. move => s s' [k1 [o1 R2]] [k0 [o0 R1]].  
+have REDS:= seqManyStep R2 R1. 
+apply: runsForLe; last first.
+eexists _, _. apply REDS. 
+rewrite addnC. apply leq_addr. 
+Qed. 
+
+Lemma properRunsTo_runsFor k : forall s s', properRunsTo s s' -> runsFor k s' -> runsFor k.+1 s. 
+Proof. move => s s' [k1 [o1 R2]] [k0 [o0 R1]].  
+have REDS:= seqManyStep R2 R1. 
+apply: runsForLe; last first.
+eexists _, _. apply REDS. 
+rewrite addnC. rewrite -(addn1 k1). rewrite (addnC k1) addnA. rewrite addn1. 
+apply leq_addr. 
+Qed. 
 
